Add slighlty modified Heap model

src/test/interop/Low_Sem.fst
@@ -1,9 +1,9 @@
 module Low_Sem
 
-module HS = FStar.HyperStack
+module M = Memory
 open Machine
 
-type mem = HS.mem
+type mem = M.heap
 
 noeq type state = {
   ok:bool;
@@ -17,3 +17,9 @@ let eval_maddr (m:maddr) (s:state) : int =
   match m with
   | MConst n -> n
   | MReg r offset -> (eval_reg r s) + offset
+
+val valid_mem: ptr:int -> h:mem -> bool
+assume val load_mem: ptr:int -> h:mem -> nat64
+assume val store_mem: ptr:int -> v:nat64 -> h:mem -> mem
+
+let valid_mem ptr h = if ptr < 0 then false else not (M.addr_unused_in ptr h)
